theories/DecSSR.v
@@ -12,17 +12,48 @@ Defined.
 
 Canonical DecBool (t : bool) := Pack (Is_true t) (dec_bool t).
 
-Definition dec_or (A B : Decidable) : decidable (A \/ B).
-  case: A=> A decA.  
-  case: B=> B decB.
-  simpl.
-  case: decA=> a.
-  left.
-  left.
-  done.
-Admitted.
+Structure EqDecidable := PackEq { type : Type; eq_dec : forall a b : type, decidable (a = b) }.
 
-Canonical Structure dec_or_can (A B : Decidable) : Decidable := Pack (A \/ B) (dec_or A B).
+Definition Decidable_eq_bool : forall (x y : bool), decidable (eq x y).
+intros. destruct x, y; try (left; done); try (right; intro H; inversion H).
+Defined.
+
+Canonical dec_eq_bool_can := PackEq bool Decidable_eq_bool.
+
+Definition Decidable_eq_nat : forall (x y : nat), decidable (eq x y).
+induction x.
+- destruct y.
+ + left ;reflexivity.
+ + right; intro H; inversion H.
+- induction y.
+  + right; intro H; inversion H.
+  + case (IHx y). intro H. left. exact (f_equal S H).
+    intro H; right. intro e. inversion e. apply (H H1).
+Defined.
+
+Canonical dec_eq_nat_can := PackEq nat Decidable_eq_nat.
+
+(* Instances for list *)
+
+Definition Decidable_eq_list : forall (HA: EqDecidable) 
+  (x y: list (type HA)), decidable (eq x y).
+intros HA. induction x.
+- destruct y.
+  + left; reflexivity.
+  + right; intro H; inversion H.
+- induction y.
+  + right; intro H; inversion H.
+  + case (eq_dec HA a a0); intro H. 
+    * case (IHx y); intro Hl.
+      left. rewrite H. rewrite Hl. reflexivity.
+      right. rewrite H. unfold not in *. 
+      intro Hc. inversion Hc. exact (Hl H1).
+    * right. unfold not in *. 
+      intro Hc. inversion Hc. exact (H H1).
+Defined.
+
+Canonical eqdec_list_can (HA: EqDecidable) 
+          := PackEq (list (type HA)) (Decidable_eq_list HA).
 
 Definition dec_le_nat : forall (x y : nat), decidable (x <= y).
 induction x.
@@ -36,3 +67,45 @@ induction x.
 Defined.
     
 Canonical Structure dec_le_nat_can (x y : nat) : Decidable := Pack (x <= y) (dec_le_nat x y).
+
+
+Definition Decidable_eq_option : forall (HA: EqDecidable) 
+  (x y: option (type HA)), decidable (eq x y).
+intros. destruct x; destruct y.
+- case (eq_dec HA t t0); intro H.
+  + left. rewrite H. reflexivity.
+  + right. unfold not in *. intro Hc. inversion Hc. 
+    exact (H H1).
+- right. unfold not. intro Hc. inversion Hc.
+- right. unfold not. intro Hc. inversion Hc.
+- left. reflexivity.
+Defined.
+
+Definition Decidable_or (HP : Decidable)
+        (HQ : Decidable) : decidable (HP \/ HQ).
+destruct HP. destruct dec0.
+- exact (left (or_introl p)).
+- destruct HQ. destruct dec0.
+  + exact (left (or_intror p)).
+  + apply right. intro H. case H; auto.
+Defined.
+    
+Canonical Structure dec_or_can (A B : Decidable) : Decidable := Pack (A \/ B) (Decidable_or A B).
+
+Definition Decidable_implies (HP : Decidable) (HQ : Decidable) : decidable (HP -> HQ).
+destruct HQ. destruct dec0.
+- exact (left (fun _ => p)).
+- destruct HP. destruct dec0.
+  + apply right. intro H. exact (n (H p)).
+  + apply left. intro p. destruct (n0 p).
+Defined.
+
+Canonical Structure dec_implies_can (HP : Decidable) (HQ : Decidable) := Pack (HP -> HQ) (Decidable_implies _ _).
+
+Canonical Structure dec_eq_option_can (HA: EqDecidable) := PackEq (option (type HA)) (Decidable_eq_option _).
+
+Canonical Structure dec_true_can := Pack True (left I).
+
+Canonical Structure dec_false_can := Pack False (right (fun x => x)).
+
+Canonical Structure dec_prove_can (P : Prop) (p : P) := Pack P (left p).
